hoist IO step / can / will / monotone / sound / complete to Smallstep
Smallstep.v now hosts: IO_event + recv/emit/step (input is total, output is
relational), allowed_trace, can_step, can_output, will_output, can_implies_will,
monotone, monotone', sound, complete, complete_weak, described_by(_weak), and
the lemmas will_implies_can, ciw_monotone, complete_weak_implies_strong.

Also weakens eventually_can_step_to_star's hypothesis from "forall t', allowed
(t' ++ t)" to just "allowed_trace t", since the proof always picks empty
demon-trace and angel-only events preserve inputs_of.

This makes everything polymorphic in (state, message, step, allowed, initial,
D), which is needed so graph-level reasoning (with message = node_id *
node_message) can reuse the node-level lemmas.

Co-Authored-By: Claude Opus 4.7 <noreply@anthropic.com>

src/util/Smallstep.v
@@ -2,60 +2,277 @@
 From Stdlib Require Import List.
 From coqutil Require Import Semantics.OmniSmallstepCombinators.
 Import ListNotations.
-Section __.
+
+Section io.
+  Context {message : Type}.
+
+  Variant IO_event : Type :=
+    | I_event : message -> IO_event
+    | O_event : list message -> IO_event.
+
+  Definition inputs_of (t : list IO_event) :=
+    flat_map (fun e => match e with I_event m => [m] | _ => [] end) t.
+
+  Definition output_in_trace (output : message) (t : list IO_event) :=
+    exists outs, In (O_event outs) t /\ In output outs.
+
+  Definition event_guaranteed (e : IO_event) :=
+    match e with
+    | O_event _ => True
+    | I_event _ => False
+    end.
+
+  Context {state : Type}.
+  Context (recv : state -> message -> state).
+  Context (emit : state -> list message -> state -> Prop).
+
+  Definition step : state -> IO_event -> state -> Prop :=
+    fun s ev s' =>
+      match ev with
+      | I_event m  => s' = recv s m
+      | O_event ms => emit s ms s'
+      end.
+End io.
+
+Arguments IO_event : clear implicits.
+
+Section star.
   Context {state event : Type} (trace := list event)
           (step : state -> event -> state -> Prop).
-Inductive star : state -> trace -> state -> Prop :=
-| star_refl s :
-  star s [] s
-| star_step s e s' t0 s'' :
-  step s e s' ->
-  star s' t0 s'' ->
-  star s (e :: t0) s''.
+  Inductive star : state -> trace -> state -> Prop :=
+  | star_refl s :
+    star s [] s
+  | star_step s e s' t0 s'' :
+    step s e s' ->
+    star s' t0 s'' ->
+    star s (e :: t0) s''.
 
-Lemma star_app s1 t1 s2 t2 s3 :
-  star s1 t1 s2 -> star s2 t2 s3 -> star s1 (t1 ++ t2) s3.
-Proof.
-  induction 1; cbn; [auto|].
-  econstructor; eauto.
-Qed.
-End __.
+  Lemma star_app s1 t1 s2 t2 s3 :
+    star s1 t1 s2 -> star s2 t2 s3 -> star s1 (t1 ++ t2) s3.
+  Proof.
+    induction 1; cbn; [auto|].
+    econstructor; eauto.
+  Qed.
+End star.
 
 Section __.
-  Context {state event : Type}.
-  Context (step : state -> event -> state -> Prop).
-  Context (allowed : list event -> Prop).
-  Context (guaranteed : list event -> event -> Prop).
+  Context {state message : Type}.
+  Context (step : state -> IO_event message -> state -> Prop).
+  Context (allowed : list message -> Prop).
+
+  Definition allowed_trace (t : list (IO_event message)) := allowed (inputs_of t).
+
+  Lemma output_in_trace_app o (l1 l2 : list (IO_event message)) :
+    output_in_trace o (l1 ++ l2) <-> output_in_trace o l1 \/ output_in_trace o l2.
+  Proof.
+    unfold output_in_trace; split.
+    - intros (outs & Hin & Hino).
+      apply in_app_or in Hin as [Hin|Hin]; [left|right]; eauto.
+    - intros [(outs & Hin & Hino)|(outs & Hin & Hino)];
+        exists outs; (split; [apply in_or_app|exact Hino]); auto.
+  Qed.
+
+  Lemma output_in_trace_rev o (l : list (IO_event message)) :
+    output_in_trace o (rev l) <-> output_in_trace o l.
+  Proof.
+    unfold output_in_trace; split; intros (outs & Hin & Hino); exists outs;
+      (split; [|exact Hino]); apply in_rev; auto.
+    rewrite rev_involutive. exact Hin.
+  Qed.
+
+  Lemma allowed_trace_universal :
+    (forall t, allowed t) -> forall t, allowed_trace t.
+  Proof. unfold allowed_trace; auto. Qed.
+
+  Lemma inputs_of_app (t1 t2 : list (IO_event message)) :
+    inputs_of (t1 ++ t2) = inputs_of t1 ++ inputs_of t2.
+  Proof. apply flat_map_app. Qed.
+
+  Lemma inputs_of_event_guaranteed (t : list (IO_event message)) :
+    Forall event_guaranteed t -> inputs_of t = [].
+  Proof.
+    induction 1; auto.
+    destruct x; cbn; auto. contradiction.
+  Qed.
+
+  Lemma output_in_trace_swap o l1 e (l2 : list (IO_event message)) :
+    output_in_trace o (l1 ++ e :: l2) <-> output_in_trace o (e :: l1 ++ l2).
+  Proof.
+    unfold output_in_trace.
+    split; intros (outs & Hin & Hino); exists outs; (split; [|exact Hino]).
+    - apply in_app_or in Hin. destruct Hin as [Hin | [Hin | Hin]].
+      + right. apply in_or_app. left. exact Hin.
+      + left. exact Hin.
+      + right. apply in_or_app. right. exact Hin.
+    - destruct Hin as [Hin | Hin].
+      + apply in_or_app. right. left. exact Hin.
+      + apply in_app_or in Hin. destruct Hin as [Hin | Hin].
+        * apply in_or_app. left. exact Hin.
+        * apply in_or_app. right. right. exact Hin.
+  Qed.
 
   (*the angel can step to the postcondition regardless of the demon's actions*)
-  Definition can_step '(s, t) (P : state * list event -> Prop) : Prop :=
+  Definition can_step '(s, t) (P : state * list (IO_event message) -> Prop) : Prop :=
     forall s' t',
       star step s t' s' ->
-      allowed (t' ++ t) ->
-      exists s'' e,
-        guaranteed (t' ++ t) e /\
-          step s' e s'' /\
-          P (s'', e :: t' ++ t).
+      allowed_trace (t' ++ t) ->
+      exists s'' outs,
+        step s' (O_event outs) s'' /\
+          P (s'', O_event outs :: t' ++ t).
 
   Lemma eventually_can_step_to_star :
-    forall (P : state * list event -> Prop) s t,
-      (forall t', allowed (t' ++ t)) ->
-      eventually (can_step) P (s, t) ->
-      exists s' tr, star step s tr s' /\ P (s', rev tr ++ t).
+    forall (P : state * list (IO_event message) -> Prop) s t,
+      allowed_trace t ->
+      eventually can_step P (s, t) ->
+      exists s' tr,
+        star step s tr s' /\
+        Forall event_guaranteed tr /\
+        P (s', rev tr ++ t).
   Proof.
     intros P s0 t0 Hallow Hwill.
     remember (s0, t0) as st eqn:Est.
     revert s0 t0 Hallow Est.
     induction Hwill as [[s' t'] HP | [s' t'] midset Hcan Hmid IH];
       intros s0 t0 Hallow [= -> ->].
-    - exists s0, []. split; [constructor|exact HP].
-    - destruct (Hcan s0 [] (star_refl _ _) (Hallow _))
-        as (s'' & e & _ & Hstep & Hmidset).
-      destruct (IH (s'', e :: t0) Hmidset s'' (e :: t0)) as (s_final & tr & Hstar & HP).
-      { intros t''. specialize (Hallow (t'' ++ [e])).
-        rewrite <- app_assoc in Hallow. exact Hallow. }
-      { reflexivity. }
-      exists s_final, (e :: tr). split; [econstructor; eassumption|].
-      cbn. rewrite <- app_assoc. exact HP.
+    - exists s0, []. split; [constructor|]. split; [constructor|exact HP].
+    - destruct (Hcan s0 [] (star_refl _ _)) as (s'' & outs & Hstep & Hmidset).
+      { cbn. exact Hallow. }
+      assert (Hallow' : allowed_trace (O_event outs :: t0)).
+      { unfold allowed_trace. cbn. exact Hallow. }
+      destruct (IH _ Hmidset s'' (O_event outs :: t0) Hallow' eq_refl)
+        as (s_final & tr & Hstar & Hguar & HP).
+      exists s_final, (O_event outs :: tr).
+      split; [econstructor; eassumption|].
+      split; [constructor; [exact I|exact Hguar]|].
+      cbn. rewrite <- app_assoc. cbn. exact HP.
+  Qed.
+
+  Definition can_output start t output :=
+    exists t' s',
+      star step start t' s' /\
+        Forall event_guaranteed t' /\
+        output_in_trace output (t' ++ t).
+
+  Definition will_output start t (output : message) : Prop :=
+    eventually can_step
+      (fun '(_, t') => output_in_trace output t')
+      (start, t).
+
+  Lemma will_implies_can :
+    forall s t o,
+      allowed_trace t ->
+      will_output s t o ->
+      can_output s t o.
+  Proof.
+    intros s0 t0 o Hall Hwill.
+    cbv [will_output] in Hwill.
+    remember (s0, t0) as st eqn:Est.
+    revert s0 t0 Hall Est.
+    induction Hwill as [[s' t'] HP | [s' t'] midset Hcan Hmid IH];
+      intros s0 t0 Hall [= -> ->].
+    - exists [], s0. split; [constructor|].
+      split; [constructor|exact HP].
+    - cbv [can_step] in Hcan.
+      specialize (Hcan s0 [] (star_refl _ _)).
+      cbn in Hcan. specialize (Hcan Hall).
+      destruct Hcan as (s'' & outs & Hstep & Hmidset).
+      assert (Hall' : allowed_trace (O_event outs :: t0)).
+      { unfold allowed_trace. cbn. exact Hall. }
+      destruct (IH _ Hmidset s'' (O_event outs :: t0) Hall' eq_refl)
+        as (t'' & s''' & Hstar'' & Hforall'' & Hout'').
+      exists (O_event outs :: t''), s'''.
+      split; [econstructor; eassumption|].
+      split; [constructor; [exact I|exact Hforall'']|].
+      cbn. apply output_in_trace_swap. exact Hout''.
+  Qed.
+
+  Context (initial : state).
+
+  Definition can_implies_will :=
+    forall t s o,
+      star step initial t s ->
+      allowed_trace t ->
+      can_output s t o ->
+      will_output s t o.
+
+  Definition monotone :=
+    forall t1 t2 s1 s2 o,
+      star step initial t1 s1 ->
+      star step s1 t2 s2 ->
+      allowed_trace t1 ->
+      allowed_trace (t2 ++ t1) ->
+      can_output s1 t1 o ->
+      can_output s2 (t2 ++ t1) o.
+
+  Definition monotone' :=
+    forall t1 t2 s1 s2 o,
+      star step initial t1 s1 ->
+      star step initial t2 s2 ->
+      incl (inputs_of t1) (inputs_of t2) ->
+      can_output s1 t1 o ->
+      can_output s2 t2 o.
+
+  Lemma ciw_monotone :
+    can_implies_will -> monotone.
+  Proof.
+    cbv [can_implies_will monotone].
+    intros Hciw t1 t2 s1 s2 o Hstar1 Hstar2 Hall1 Hallt Hcan.
+    apply (Hciw _ _ _ Hstar1 Hall1) in Hcan.
+    cbv [will_output] in Hcan.
+    inversion Hcan as [HP | midset Hcan_step Hmid]; clear Hcan; subst.
+    - exists [], s2. split; [constructor|].
+      split; [constructor|].
+      cbn. apply output_in_trace_app. right. exact HP.
+    - cbv [can_step] in Hcan_step.
+      specialize (Hcan_step _ _ Hstar2 Hallt).
+      destruct Hcan_step as (s'' & outs & Hstep & Hmidset).
+      specialize (Hmid _ Hmidset).
+      assert (Hall' : allowed_trace (O_event outs :: t2 ++ t1)).
+      { unfold allowed_trace. cbn. exact Hallt. }
+      apply (will_implies_can _ _ _ Hall') in Hmid.
+      destruct Hmid as (t' & s''' & Hstar' & Hforall' & Hout').
+      exists (O_event outs :: t'), s'''.
+      split; [econstructor; eassumption|].
+      split; [constructor; [exact I|exact Hforall']|].
+      cbn. apply output_in_trace_swap. exact Hout'.
+  Qed.
+
+  Context (D : list message -> message -> Prop).
+
+  Definition complete :=
+    forall t s,
+      star step initial t s ->
+      allowed_trace t ->
+      forall output,
+        D (inputs_of t) output ->
+        will_output s t output.
+
+  Definition sound :=
+    forall t s,
+      star step initial t s ->
+      allowed_trace t ->
+      forall output,
+        output_in_trace output t ->
+        D (inputs_of t) output.
+
+  Definition described_by := sound /\ complete.
+
+  Definition complete_weak :=
+    forall t s,
+      star step initial t s ->
+      allowed_trace t ->
+      forall output,
+        D (inputs_of t) output ->
+        can_output s t output.
+
+  Definition described_by_weak := sound /\ complete_weak.
+
+  Lemma complete_weak_implies_strong :
+    complete_weak ->
+    can_implies_will ->
+    complete.
+  Proof.
+    intros Hweak Hcan t s Hstar Hall o HD.
+    apply Hcan; auto.
   Qed.
 End __.
